2 and 5

lesson5.v
@@ -7,38 +7,91 @@ Unset Printing Implicit Defensive.
 ----------------------------------------------------------
 #<div class="slide">#
 
-** Reflection in the large (and small?)
+** Reflection in the large
 
-some text
+*** In this lecture
+  - bla
+  - bla
 
-#<a href="https://example.com">some html link</a>#
 
-This is inline Coq code [fun x => x] and now some block Coq code
+#</div>#
+----------------------------------------------------------
+#<div class="slide vfill">#
+
+** Recap: computation and variables
+
+- Why is the first goal trivial by computation?
+- Why the second is not?
 
 #<div>#
 *)
-
 Lemma ex1 x : 0 * x = 0.
-by []. Qed.
+Proof. by []. Qed.
 
 Lemma ex2 x : x * 0 = 0.
+Proof.
 Fail by [].
 Admitted.
 
-Module A.
+(**
+#</div>#
+
+We used the lemma [muln0] before. Can't we explain Coq
+to use it for us?
+
+#</div>#
+----------------------------------------------------------
+#<div class="slide">#
+
+*** Idea
+   - we could write a program that simplifies expressions
+   - we could provide it correct
+   - we could have Coq run it for us
+
+#<div>#
+*)
+Module A. (* A module is a box for Coq code, ignore this *)
 
 Inductive expr :=
   | Zero
   | Mult (x : expr) (y : expr)
   | Extra (stuff : nat).
+(**
+#</div>#
+
+The [expr] data type is the _syntax_ of expressions.
+It is a data type like [nat] or [bool] are we know how to
+write programs on this data.
+
+Let's write a program that deal with Zero.
+
+#<div>#
+*)
 
 Fixpoint simplify e :=
   match e with
-  | Mult Zero x => Zero
-  | Mult x Zero => Zero
-  | y => y
+  | Mult x y =>
+      match simplify x, simplify y with
+      | Zero, _ => Zero
+      | _, Zero => Zero
+      | a, b => Mult a b
+      end
+  | x => x
   end.
 
+(* Syntax of (3 * 0) * 4 *)
+Definition T : expr := Mult (Mult (Extra 3) Zero) (Extra 4).
+
+Eval lazy in simplify T. (* = Zero *)
+(**
+#</div>#
+
+We have to link these expressions and out goals.
+Each expression in [expr] represents an expression in out goal.
+Let's make this map explicit.
+
+#<div>#
+*)
 Fixpoint interp e :=
   match e with
   | Zero => 0
@@ -46,38 +99,102 @@ Fixpoint interp e :=
   | Extra x => x
   end.
 
-Lemma go e : interp e = interp (simplify e).
-have im a b : interp (Mult a b) = (interp a) * (interp b) by [].
-elim: e => //= - [//|x y Hxy|e He] [|a b Hab|f Hf]; by [ rewrite muln0 | rewrite -im ].
+Eval lazy delta [T interp] iota beta in interp T.
+(**
+#</div>#
+
+What would it mean for [simplify] to be correct?
+
+#<div>#
+*)
+
+Lemma simplify_correct (e : expr) : interp e = interp (simplify e).
+Proof.
+have interpMult a b : interp (Mult a b) = (interp a) * (interp b) by [].
+elim: e => //=.
+move=> x Hx y Hy.
+case Ex : (simplify x) => [|x1 x2|n].
+- by rewrite Hx Ex. (* 0 * n = n by computation *)
+- case Ey : (simplify y) => [|y1 y2|m].
+  + by rewrite Hy Ey /= muln0. (* n * 0 = 0 by muln0 *)
+  + by rewrite Hx Hy Ex Ey -interpMult.
+  + by rewrite Hx Hy Ex Ey -interpMult.
+- case Ey: (simplify y)  => [|y1 y2|m].
+  + by rewrite Hy Ey muln0. (* n * 0 = 0 by muln0 *)
+  + by rewrite Hx Hy Ex Ey -interpMult.
+  + by rewrite Hx Hy Ex Ey -interpMult.
 Qed.
 
+(**
+#</div>#
+
+Now let's take advantage of 
+
+#<div>#
+*)
 
 Lemma ex3 x : x * 0 = 0.
 Proof.
-rewrite -[LHS]/(interp (Mult (Extra x) Zero)).
-rewrite go.
+pose AST : expr := Mult (Extra x) Zero.
+rewrite -[LHS]/(interp AST).
+rewrite simplify_correct.
 rewrite /=.
 by [].
-Defined.
-
-Eval lazy delta [ex3] beta in ex3.
+Qed.
 
 End A.
+(**
+#</div>#
 
+#</div>#
+----------------------------------------------------------
+#<div class="slide">#
+
+*** Let's add more simplification rules!
+
+#<div>#
+*)
 Module B.
 
 Inductive expr :=
   | Zero
   | Minus (x : expr) (y : expr)
-  | Extra (n : nat).
+  | Extra (stuff : nat).
+(**
+#</div>#
 
-  Fixpoint simplify e :=
+The rule we want is #$n - n = 0$# when n is a number
+
+#<div>#
+*)
+
+Fixpoint simplify e :=
   match e with
-  | Minus (Extra x) (Extra y) =>
-       match eqn x y with true => Zero | _ => e end
-  | y => y
+  | Minus x y =>
+      match simplify x, simplify y with
+      | Extra n, Extra m =>
+          match n == m with
+          | true => Zero
+          | false => Minus (Extra n) (Extra m)
+          end
+      | a, b => Minus a b
+      end
+  | x => x
   end.
 
+(* Syntax of (3 - 3 *)
+Definition T : expr := Minus (Extra 3) (Extra 3).
+
+Eval lazy in simplify T. (* = Zero *)
+(**
+#</div>#
+
+We have to link these expressions and out goals.
+Each expression in [expr] represents an expression in out goal.
+Let's make this map explicit.
+
+#<div>#
+*)
 Fixpoint interp e :=
   match e with
   | Zero => 0
@@ -85,54 +202,119 @@ Fixpoint interp e :=
   | Extra x => x
   end.
 
-Lemma go e : interp e = interp (simplify e).
-have im a b : interp (Minus a b) = (interp a) - (interp b) by [].
-elim: e => //= - [//|x y Hxy|e He] [|a b Hab|f Hf]; try by rewrite -im.
-by rewrite /=; case: eqnP => //= ->; rewrite subnn.
+Eval lazy delta [T interp] iota beta in interp T.
+(**
+#</div>#
+
+What would it mean for [simplify] to be correct?
+
+#<div>#
+*)
+
+Lemma simplify_correct (e : expr) : interp e = interp (simplify e).
+Proof.
+have interpMinus a b : interp (Minus a b) = (interp a) - (interp b) by [].
+elim: e => //=.
+move=> x Hx y Hy.
+  case Ex : (simplify x) => [|x1 x2|n].
+  - by rewrite Hx Ex.
+  - by rewrite Hx Ex Hy.
+  - case Ey : (simplify y) => [|y1 y2|m].
+    + by rewrite Hx Hy Ex Ey -interpMinus.
+    + by rewrite Hx Hy Ex Ey -interpMinus.
+    + case: eqP.
+      + by rewrite Hx Hy Ex Ey => ->; rewrite subnn.
+      + by rewrite Hx Hy Ex Ey -interpMinus.
 Qed.
 
+(**
+#</div>#
+
+Now let's try to take advantage of it
+
+#<div>#
+*)
 
 Lemma ex3 x : x - x = 0.
 Proof.
-rewrite -[LHS]/(interp (Minus (Extra x) (Extra x))).
-rewrite go.
+pose AST : expr := Minus (Extra x) (Extra x).
+rewrite -[LHS]/(interp AST).
+rewrite simplify_correct.
 rewrite /=.
 Abort.
 
+
 End B.
+(**
+#</div>#
+
+What went wrong...
+
+#</div>#
+----------------------------------------------------------
+#<div class="slide">#
+
+*** Let's add more simplification rules!
+
+#<div>#
+*)
 
 Module C.
 
 Inductive expr :=
   | Zero
   | Minus (x : expr) (y : expr)
-  | Extra (n : nat).
+  | ExtraId (n : nat).
 
-  Fixpoint simplify e :=
+Fixpoint simplify e :=
   match e with
-  | Minus (Extra x) (Extra y) =>
-       match eqn x y with true => Zero | _ => e end
+  | Minus x y =>
+      match simplify x, simplify y with
+      | ExtraId n, ExtraId m =>
+          match n == m with
+          | true => Zero
+          | false => Minus (ExtraId n) (ExtraId m)
+          end
+      | a, b => Minus a b
+      end
   | y => y
   end.
 
-Fixpoint interp e c :=
+Fixpoint interp (e : expr) (c : list nat) :=
   match e with
   | Zero => 0
   | Minus x y => (interp x c) - (interp y c)
-  | Extra x => nth 0 c x
+  | ExtraId x => nth 0 c x
   end.
 
-Lemma go e ct : interp e ct = interp (simplify e) ct.
-have im a b c : interp (Minus a b) c = (interp a c) - (interp b c) by [].
-elim: e => //= - [//|x y Hxy|e He] [|a b Hab|f Hf]; try by rewrite -im.
-by rewrite /=; case: eqnP => //= ->; rewrite subnn.
+  (* Syntax of (3 - 3 *)
+Definition T : expr := Minus (ExtraId 0) (ExtraId 0).
+Definition C : list nat := [:: 3].
+Eval lazy delta [T C interp nth] iota beta in interp T C.
+
+
+Lemma simplify_correct (e : expr) (c : list nat) : interp e c = interp (simplify e) c.
+Proof.
+have interpMinus a b l : interp (Minus a b) l = (interp a l) - (interp b l) by [].
+elim: e => //=.
+move=> x Hx y Hy.
+  case Ex : (simplify x) => [|x1 x2|n].
+  - by rewrite Hx Ex.
+  - by rewrite Hx Ex Hy.
+  - case Ey : (simplify y) => [|y1 y2|m].
+    + by rewrite Hx Hy Ex Ey -interpMinus.
+    + by rewrite Hx Hy Ex Ey -interpMinus.
+    + case: eqP.
+      + by rewrite Hx Hy Ex Ey => ->; rewrite subnn.
+      + by rewrite Hx Hy Ex Ey -interpMinus.
 Qed.
 
 Lemma ex3 x : x - x = 0.
 Proof.
-pose AST : expr := Minus (Extra 0) (Extra 0).
-rewrite -[LHS]/(interp AST [::x]).
-rewrite go.
+pose AST : expr := Minus (ExtraId 0) (ExtraId 0).
+pose CTX : list nat := [:: x].
+rewrite -[LHS]/(interp AST CTX).
+rewrite simplify_correct.
 rewrite /=.
 by [].
 Qed.
@@ -148,20 +330,6 @@ Qed.
 
 (**
 #</div>#
-
-You cna also put latex math here
-
-#$$ \
-
-{i=1}^n (i * 2 - 1) = n ^ 2 $$#
-
-finally some notes, hover to unravel
-
-#<div class="note">(notes)<div class="note-text">#
-You don't need to install Coq in order to follow this
-class, you just need a recent browser thanks to
-#<a href="https://github.com/ejgallego/jscoq">jsCoq</a>#.
-#</div></div>#
 
 #</div>#
 ----------------------------------------------------------
