exercise2.v
@@ -1,81 +1,147 @@
-From mathcomp Require Import all_ssreflect.
+(* ignore these directives *)
+From mathcomp Require Import mini_ssreflect.
 Set Implicit Arguments.
 Unset Strict Implicit.
 Unset Printing Implicit Defensive.
+Add Printing Coercion is_true.
+Notation "x '= true'" := (is_true x) (x at level 100, at level 0, only printing).
+Remove Printing If bool.
 
-(** *** Exercise :
+(** *** Exercise 1:
+  - Define a function double that takes a natural
+    number to its double.
+  - you can use the operations on nat that we dinefined in class
+*)
+Definition double (n : nat) : nat := (* fill this in *)
+(*D*)2 * n.
+
+Eval lazy in double 3. (* = 6 *)
+
+(** *** Exercise 2:
+   - Define a function that takes a natural number and tests
+     if it is zero. In that case the value of the function is 1,
+     otherwise it is the double of the given number.
+   - The skeleton of the function is given, fill in the blanks. *)
+Infix "==" := eqn. (* recall, infix == tests for equality *)
+Definition double_z (n : nat) : nat :=
+  match
+    (* fill this in *)
+(*D*)n == 0
+  with
+  | true => (* fill this in*)
+(*D*) 1
+  | false => (* fill this in *)
+(*D*) double n
+  end.
+
+Eval lazy in double_z 0. (* = 1 *)
+Eval lazy in double_z 4. (* = 8 *)
+
+(** *** Exercise 3:
+   - Define boolean negation. We did peek at it during the lesson,
+     now try to write it yourself.
+*)
+Definition negb (b : bool) : bool := (* fill this in *)
+(*D*)match b with true => false | false => true end.
+
+Eval lazy in negb true. (* = false *)
+Eval lazy in negb false. (* = true *)
+
+(** *** Exercise 4:
+   - write the Fibonacci function (growth of a rabbit population).
+     #$$ \phi(n) = \begin{array}{|c}1~\mathrm{if}~n = 0 \\ 1~\mathrm{if}~n = 1\\ \phi(n-1) + \phi(n-2)~\mathrm{otherwise}\end{array} $$#
+*)
+Fixpoint fibonacci (n : nat) : nat :=
+  match n with
+  | 0 => (* fill this in *)
+(*D*)  1
+  | 1 => (* fill this in *)
+(*D*) 1
+  | S p => (* fill this in, hint: think at the relation between n and p *)
+(*D*) fibonacci p + fibonacci (p - 1)
+  end.
+
+Eval lazy in fibonacci 3. (* = 3*)
+Eval lazy in fibonacci 7. (* = 21 *)
+Eval lazy in fibonacci 10. (* = 89 *)
+
+
+(** *** Exercise 5:
     - Define the option container with constructors None and Some
     - Define the "projection" default
 *)
-Inductive option
-(*D*)A := Some (a : A) | None.
+Inductive option A :=
+| Some (* fill this in *)
+(*D*)(a : A)
+| None.
+
+(* Ignore these directives *)
 Arguments Some {_}.
 Arguments None {_}.
 
-Definition default
-(*D*)A (a : A) (x : option A) := if x is Some v then v else a.
-Eval lazy in default 3 None. (* 3 *)
-Eval lazy in default 3 (Some 4). (* 4 *)
+Definition default A (a : A) (x : option A) : A := (* fill this in *)
+(*D*)match x with Some v => v | None => a end.
 
-(** *** Exercise :
-    Define boolean negation
-*)
-Definition negb b :=
-(*D*)if b then false else true.
-Notation "~~ x" := (negb x).
+Eval lazy in default 3 None. (* = 3 *)
+Eval lazy in default 3 (Some 4). (* = 4 *)
 
-Eval lazy in negb true.
-Eval lazy in negb false.
-
-(** *** Exercise :
+(** *** Exercise 6:
     Use the [iter] function below to define:
     - addition over natural numbers.
     - multiplication over natural unmbers.
 *)
-Fixpoint iter (T : Type) n op (x : T) :=
-  if n is p.+1 then op (iter p op x) else x.
+Fixpoint iter T (n : nat) (op : T -> T) (x : T) : T :=
+  match n with
+  | 0 => x
+  | S p => op (iter p op x)
+  end.
+(* Ignore this directive *)
 Arguments iter {T}.
 
-Definition addn n m :=
+Definition addn (n : nat) (m : nat) : nat := (* fill this in *)
 (*D*)iter n S m.
 
 Eval lazy in addn 3 4.
 
-Definition muln n m :=
+Definition muln (n : nat) (m : nat) : nat := (* fill this in *)
 (*D*)iter n (addn m) 0.
 
 Eval lazy in muln 3 4.
 
-(** *** Exercise :
-    - Define muln by recursion
+(** *** Exercise 7:
+    - prove the following statement by case split
 *)
-Fixpoint muln_rec n m :=
-(*D*)if n is p.+1 then m + (muln_rec p m) else 0.
-(** Cheat sheet available at
-      #<a href='https://www-sop.inria.fr/teams/marelle/types18/cheatsheet.pdf'>https://www-sop.inria.fr/teams/marelle/types18/cheatsheet.pdf</a>#
+Lemma orbC (p : bool) (q : bool) : p || q = q || p.
+Proof.
+(* fill this in *)
+(*D*)by case: p; case: q.
+Qed.
+
+(** *** Exercise 8:
+   - look up what [==>] is and prove the Peirce law
 *)
+Locate "fill this in".
+Print (* the name behind ==> *)
+(*D*)implb.
+Lemma Peirce (p : bool) (q : bool) : ((p ==> q) ==> p) ==> p.
+Proof.
+(* fill this in *)
+(*D*)by case: p; case: q.
+Qed.
 
-Implicit Type p q r : bool.
-Implicit Type m n a b c : nat.
-
-(** *** Exercise 1:
-    - use no lemma to prove the following statement
-*)
-Lemma orbC p q : p || q = q || p.
-(*D*)Proof. by case: p; case: q. Qed.
-
-(** *** Exercise 2:
-   - look up what [==>] is and prove that as you like
-*)
-Lemma Peirce p q : ((p ==> q) ==> p) ==> p.
-(*D*)Proof. by case: p; case: q. Qed. 
-
-(** *** Exercise 3:
+(** *** Exercise 9:
     - what is [(+)] ?
-    - prove this using move and rewrite
+    - Hint: [->] in the goal stands for implication, use move to name the
+      assumption
+    - Hint: use Search to dind useful lemmas and use rewrite to use them
 *)
-Lemma find_me p q :  ~~ p = q -> p (+) q.
-(*D*)Locate "(+)".
-(*D*)Search _ addb negb.
-(*D*)Proof. by move=> np_q; rewrite -np_q addbN negb_add. Qed.
+Locate (* fill this in *)
+(*D*)"(+)".
+Search _ (* fil this in*)
+(*D*)(_ (+) ~~ _).
+Lemma find_me (p : bool) (q : bool) :  ~~ p = q -> p (+) q.
+Proof.
+(* fill this in *)
+(*D*)by move=> np_q; rewrite -np_q addbN negb_add.
+Qed.
 
